# Pre-Calculus Section Sheet
## First Year University - Non-Math Basics

---

## Table of Contents
1. Mathematical Symbols and Notation
2. Real Line
3. Properties of Real Numbers
4. Order Relations and Intervals
5. Exponents and Radicals
6. Algebraic Identities
7. Practice Problems with Solutions

---

## 1. Mathematical Symbols and Notation (الرموز الرياضية)

### Basic Symbols

| Symbol | Name (English) | Name (Arabic) | Meaning |
|--------|----------------|---------------|---------|
| + | Plus | زائد | Addition |
| − | Minus | ناقص | Subtraction |
| × or · | Times | ضرب | Multiplication |
| ÷ or / | Divided by | قسمة | Division |
| = | Equals | يساوي | Equality |
| ≠ | Not equal | لا يساوي | Inequality |
| < | Less than | أصغر من | Comparison |
| > | Greater than | أكبر من | Comparison |
| ≤ | Less than or equal | أصغر من أو يساوي | Comparison |
| ≥ | Greater than or equal | أكبر من أو يساوي | Comparison |

### Advanced Symbols

| Symbol | Name (English) | Name (Arabic) | Meaning |
|--------|----------------|---------------|---------|
| √ | Square root | الجذر التربيعي | Root extraction |
| ∛ | Cube root | الجذر التكعيبي | Cube root |
| ⁿ√ | nth root | الجذر النوني | nth root |
| ∞ | Infinity | ما لا نهاية | Unbounded |
| ∈ | Element of | ينتمي إلى | Set membership |
| { } | Set brackets | أقواس المجموعة | Set notation |
| [ ] | Closed bracket | قوس مغلق | Interval notation |
| ( ) | Open bracket | قوس مفتوح | Interval notation |
| : | Such that | بحيث | Condition |

---

## 2. Real Line (الخط الحقيقي)

### Definition (التعريف)
The **real line** is a geometric representation where every real number corresponds to exactly one point on an infinite straight line, and every point on the line corresponds to exactly one real number.

### Key Concepts (المفاهيم الأساسية)

**One-to-One Correspondence (التطابق الأحادي):**
- Each real number ↔ Exactly one point on the line
- Each point on the line ↔ Exactly one real number

### Visual Representation

```
        -3      -2      -1       0       1       2       3
         |-------|-------|-------|-------|-------|-------|------>
    (negative)                          (positive)
```

### Important Points (نقاط مهمة)
- **Origin (نقطة الأصل):** The point 0 on the line
- **Positive direction (الاتجاه الموجب):** To the right of 0
- **Negative direction (الاتجاه السالب):** To the left of 0

---

## 3. Properties of Real Numbers (خصائص الأعداد الحقيقية)

For any real numbers **a**, **b**, and **c**:

### 3.1 Commutative Property (الخاصية التبديلية)

**Addition (الجمع):**
- **a + b = b + a**
- Example: 3 + 5 = 5 + 3 = 8

**Multiplication (الضرب):**
- **a · b = b · a**
- Example: 4 × 7 = 7 × 4 = 28

---

### 3.2 Associative Property (الخاصية التجميعية)

**Addition (الجمع):**
- **(a + b) + c = a + (b + c)**
- Example: (2 + 3) + 4 = 2 + (3 + 4)
  - Left side: 5 + 4 = 9
  - Right side: 2 + 7 = 9

**Multiplication (الضرب):**
- **(a · b) · c = a · (b · c)**
- Example: (2 × 3) × 4 = 2 × (3 × 4)
  - Left side: 6 × 4 = 24
  - Right side: 2 × 12 = 24

---

### 3.3 Identity Property (خاصية المحايد)

**Additive Identity (المحايد الجمعي):**
- **a + 0 = a = 0 + a**
- 0 is called the **additive identity (المحايد الجمعي)**
- Example: 7 + 0 = 7

**Multiplicative Identity (المحايد الضربي):**
- **a · 1 = a = 1 · a**
- 1 is called the **multiplicative identity (المحايد الضربي)**
- Example: 9 × 1 = 9

---

### 3.4 Inverse Property (خاصية المعكوس)

**Additive Inverse (المعكوس الجمعي):**
- **a + (−a) = 0 = (−a) + a**
- −a is called the **additive inverse (المعكوس الجمعي)** of a
- Example: 5 + (−5) = 0

**Multiplicative Inverse (المعكوس الضربي):**
- **a · (1/a) = 1 = (1/a) · a** (where a ≠ 0)
- 1/a is called the **multiplicative inverse (المعكوس الضربي)** or **reciprocal (المقلوب)** of a
- Example: 4 × (1/4) = 1

---

### 3.5 Distributive Property (خاصية التوزيع)

**a(b + c) = ab + ac** and **(b + c)a = ba + ca**

**Example 1:**
Expand: 3(x + 4)

**Solution:**
- 3(x + 4) = 3·x + 3·4
- = 3x + 12

**Example 2:**
Expand: 5(2y − 3)

**Solution:**
- 5(2y − 3) = 5·2y + 5·(−3)
- = 10y − 15

---

## 4. Order Relations and Intervals (علاقات الترتيب والفترات)

### 4.1 Order Relations (علاقات الترتيب)

| Notation | Terminology | Meaning |
|----------|-------------|---------|
| a < b | a is less than b (أصغر من) | b = a + d, for some positive number d |
| b > a | b is greater than a (أكبر من) | Same as a < b |
| a ≤ b | a is less than or equal to b (أصغر من أو يساوي) | a < b or a = b |
| b ≥ a | b is greater than or equal to a (أكبر من أو يساوي) | Same as a ≤ b |

**Examples:**
- 3 < 7 (3 is less than 7)
- −2 < 0 (negative 2 is less than 0)
- 5 ≥ 5 (5 is greater than or equal to 5)
- 10 ≥ 8 (10 is greater than or equal to 8)

---

### 4.2 Intervals (الفترات)

Intervals are sets of real numbers between (or beyond) certain values.

#### Types of Intervals:

**1. Open Interval (الفترة المفتوحة):**
- **Notation:** ]a, b[ or (a, b)
- **Set Description:** {x: a < x < b}
- **Meaning:** All numbers between a and b, **not including** a and b
- **Picture:** ◯————————◯
- **Example:** ]2, 5[ includes 2.1, 3, 4.9 but NOT 2 or 5

---

**2. Closed Interval (الفترة المغلقة):**
- **Notation:** [a, b]
- **Set Description:** {x: a ≤ x ≤ b}
- **Meaning:** All numbers between a and b, **including** a and b
- **Picture:** ●————————●
- **Example:** [2, 5] includes 2, 2.1, 3, 4.9, and 5

---

**3. Half-Closed Interval (الفترة نصف المغلقة):**

**Type A: Closed on left, open on right**
- **Notation:** [a, b[
- **Set Description:** {x: a ≤ x < b}
- **Meaning:** Includes a but NOT b
- **Picture:** ●————————◯
- **Example:** [2, 5[ includes 2, 3, 4.9 but NOT 5

**Type B: Half-Open Interval (الفترة نصف المفتوحة):**
- **Notation:** ]a, b]
- **Set Description:** {x: a < x ≤ b}
- **Meaning:** Includes b but NOT a
- **Picture:** ◯————————●
- **Example:** ]2, 5] includes 3, 4.9, 5 but NOT 2

---

**4. Infinite Intervals (الفترات اللانهائية):**

**Type A: x > a (open)**
- **Notation:** ]a, ∞[
- **Set Description:** {x: x > a}
- **Picture:** ◯—————→
- **Example:** ]3, ∞[ includes 4, 100, 1000, ... but NOT 3

**Type B: x ≥ a (closed)**
- **Notation:** [a, ∞[
- **Set Description:** {x: x ≥ a}
- **Picture:** ●—————→
- **Example:** [3, ∞[ includes 3, 4, 100, 1000, ...

**Type C: x < b (open)**
- **Notation:** ]−∞, b[
- **Set Description:** {x: x < b}
- **Picture:** ←—————◯
- **Example:** ]−∞, 5[ includes 4, 0, −100, ... but NOT 5

**Type D: x ≤ b (closed)**
- **Notation:** ]−∞, b]
- **Set Description:** {x: x ≤ b}
- **Picture:** ←—————●
- **Example:** ]−∞, 5] includes 5, 4, 0, −100, ...

---

### Important Notes (ملاحظات مهمة):
- The symbol **∞** (infinity - ما لا نهاية) does NOT represent a real number
- We **NEVER** use a closed bracket [ or ] with ∞
- Always use open bracket ( or ) with ∞

---

## 5. Exponents and Radicals (الأسس والجذور)

### 5.1 Basic Terminology (المصطلحات الأساسية)

**Exponential Expression:** aⁿ

- **Base (الأساس):** The number **a** being multiplied
- **Exponent (الأس):** The number **n** indicating how many times to multiply
- **Power (القوة):** The entire expression **aⁿ**
- **Degree (الدرجة):** The value of the exponent

**Example:** In 2³:
- Base = 2
- Exponent = 3
- Power = 2³ = 8
- Meaning: 2 × 2 × 2 = 8

---

### 5.2 Rules of Exponents (قوانين الأسس)

#### **1. Product Rule (قانون الضرب)**
**aᵐ · aⁿ = aᵐ⁺ⁿ**

When multiplying powers with the same base, **add** the exponents.

**Example:**
- 2³ · 2⁵ = 2³⁺⁵ = 2⁸
- Verification: (2×2×2) · (2×2×2×2×2) = 2⁸ = 256

---

#### **2. Quotient Rule (قانون القسمة)**
**aᵐ / aⁿ = aᵐ⁻ⁿ**

When dividing powers with the same base, **subtract** the exponents.

**Example:**
- 2⁵ / 2² = 2⁵⁻² = 2³ = 8
- Verification: 32 / 4 = 8 ✓

---

#### **3. Power of a Product Rule (قانون قوة الضرب)**
**(ab)ᵐ = aᵐbᵐ**

**Example:**
- (3 × 4)² = 3² × 4² = 9 × 16 = 144
- Verification: (12)² = 144 ✓

---

#### **4. Power of a Power Rule (قانون قوة الأس)**
**(aᵐ)ⁿ = aᵐⁿ**

**Example:**
- (2³)⁴ = 2³ˣ⁴ = 2¹² = 4096

---

#### **5. Power of a Quotient Rule (قانون قوة القسمة)**
**(a/b)ⁿ = aⁿ/bⁿ** (where b ≠ 0)

**Example:**
- (3/4)² = 3²/4² = 9/16

---

#### **6. Negative Exponent Rule (قانون الأس السالب)**
**a⁻ᵐ = 1/aᵐ** (where a ≠ 0)

**Example:**
- 2⁻³ = 1/2³ = 1/8

---

#### **7. Zero Exponent Rule (قانون الأس الصفري)**
**a⁰ = 1** (where a ≠ 0)

**Example:**
- 5⁰ = 1
- 100⁰ = 1
- (−7)⁰ = 1

---

#### **8. Fractional Exponents (الأسس الكسرية)**
**a^(m/n) = ⁿ√(aᵐ)**

The numerator (m) is the power, the denominator (n) is the root.

**Example:**
- 8^(2/3) = ³√(8²) = ³√64 = 4
- OR: 8^(2/3) = (³√8)² = 2² = 4

---

### 5.3 Radicals (الجذور)

**Radical Expression:** ⁿ√a

- **Radical Sign (علامة الجذر):** √ or ⁿ√
- **Radicand (العدد تحت الجذر):** The number **a** under the radical
- **Index (الدليل):** The number **n** indicating which root (if not shown, n = 2)

**Examples:**
- √16 = 4 (square root - الجذر التربيعي)
- ³√8 = 2 (cube root - الجذر التكعيبي)
- ⁴√16 = 2 (fourth root - الجذر الرابع)

---

### 5.4 Practice Examples with Exponents

**Example 1:** Simplify x⁶x⁻³

**Solution:**
- Step 1: Apply product rule: x⁶x⁻³ = x⁶⁺⁽⁻³⁾
- Step 2: Simplify exponent: x⁶⁻³ = x³
- **Answer: x³**

---

**Example 2:** Simplify (x⁻¹y²)/(z⁻³)

**Solution:**
- Step 1: Apply negative exponent rule: x⁻¹ = 1/x and z⁻³ = 1/z³
- Step 2: Rewrite: (y²/x)/(1/z³)
- Step 3: Division becomes multiplication: (y²/x) × z³
- Step 4: Simplify: (y²z³)/x
- **Answer: y²z³/x**

---

**Example 3:** Simplify (x⁻²y³)⁴

**Solution:**
- Step 1: Apply power of a power rule to each term: (x⁻²)⁴(y³)⁴
- Step 2: Multiply exponents: x⁻⁸y¹²
- Step 3: Apply negative exponent rule: y¹²/x⁸
- **Answer: y¹²/x⁸**

---

**Example 4:** Simplify (2x²)⁻³ · y⁴ ÷ (x⁻¹y)²

**Solution:**
- Step 1: Simplify (2x²)⁻³
  - (2x²)⁻³ = 2⁻³(x²)⁻³ = (1/8)x⁻⁶ = 1/(8x⁶)

- Step 2: Simplify (x⁻¹y)²
  - (x⁻¹y)² = (x⁻¹)²(y)² = x⁻²y²

- Step 3: Rewrite the expression:
  - [1/(8x⁶)] · y⁴ ÷ [x⁻²y²]
  - = [y⁴/(8x⁶)] ÷ [y²/x²]

- Step 4: Division becomes multiplication by reciprocal:
  - = [y⁴/(8x⁶)] × [x²/y²]

- Step 5: Simplify:
  - = (y⁴ · x²)/(8x⁶ · y²)
  - = x²y⁴/(8x⁶y²)
  - = y²/(8x⁴)

- **Answer: y²/(8x⁴)**

---

## 6. Algebraic Identities (المتطابقات الجبرية)

### 6.1 Important Definitions (تعريفات مهمة)

**Identity (المتطابقة):** An equation that is true for all values of the variables.

**Factor (العامل):** Numbers or expressions that are multiplied together.

**Expand (التوسيع):** To multiply out and remove parentheses.

**Factorize (التحليل):** To write as a product of factors.

---

### 6.2 Basic Identities (المتطابقات الأساسية)

#### **Identity 1: Square of a Sum (مربع المجموع)**
**(a + b)² = a² + 2ab + b²**

**NOT equal to a² + b²** ⚠️

**Example 1:** Expand (2x + 3)²

**Solution:**
- Step 1: Identify a = 2x, b = 3
- Step 2: Apply formula: (2x)² + 2(2x)(3) + (3)²
- Step 3: Simplify: 4x² + 12x + 9
- **Answer: 4x² + 12x + 9**

---

#### **Identity 2: Square of a Difference (مربع الفرق)**
**(a − b)² = a² − 2ab + b²**

**NOT equal to a² − b²** ⚠️

**Example 2:** Expand (3x − y)²

**Solution:**
- Step 1: Identify a = 3x, b = y
- Step 2: Apply formula: (3x)² − 2(3x)(y) + (y)²
- Step 3: Simplify: 9x² − 6xy + y²
- **Answer: 9x² − 6xy + y²**

---

#### **Identity 3: Difference of Squares (الفرق بين مربعين)**
**(a + b)(a − b) = a² − b²**

**Example 3:** Expand (x + 3y)(x − 3y)

**Solution:**
- Step 1: Identify a = x, b = 3y
- Step 2: Apply formula: x² − (3y)²
- Step 3: Simplify: x² − 9y²
- **Answer: x² − 9y²**

---

#### **Identity 4: Product of Two Binomials (ضرب حدين)**
**(a + b)(c + d) = ac + ad + bc + bd**

**FOIL Method:** First, Outer, Inner, Last

**Example 4:** Expand (x + 3y)(x + 4y)

**Solution:**
- Step 1: First: x · x = x²
- Step 2: Outer: x · 4y = 4xy
- Step 3: Inner: 3y · x = 3xy
- Step 4: Last: 3y · 4y = 12y²
- Step 5: Combine: x² + 4xy + 3xy + 12y²
- Step 6: Simplify: x² + 7xy + 12y²
- **Answer: x² + 7xy + 12y²**

---

### 6.3 Special Cases with Radicals

**Example 5:** Expand (2√x − 3)²

**Solution:**
- Step 1: Identify a = 2√x, b = 3
- Step 2: Apply (a − b)² = a² − 2ab + b²
- Step 3: (2√x)² − 2(2√x)(3) + (3)²
- Step 4: 4x − 12√x + 9
- **Answer: 4x − 12√x + 9**

---

**Example 6:** Expand (√x + 5)(√x − 5)

**Solution:**
- Step 1: Identify a = √x, b = 5
- Step 2: Apply (a + b)(a − b) = a² − b²
- Step 3: (√x)² − (5)²
- Step 4: x − 25
- **Answer: x − 25**

---

### 6.4 Factorization (التحليل إلى عوامل)

Factorization is the reverse process of expansion.

**Example 7:** Factorize x² − 7x + 12

**Solution:**
- Step 1: Find two numbers that multiply to +12 and add to −7
- Step 2: The numbers are −3 and −4
  - (−3) × (−4) = 12 ✓
  - (−3) + (−4) = −7 ✓
- Step 3: Write as factors: (x − 3)(x − 4)
- **Answer: (x − 3)(x − 4)**

---

**Example 8:** Factorize x² + x − 6

**Solution:**
- Step 1: Find two numbers that multiply to −6 and add to +1
- Step 2: The numbers are +3 and −2
  - (+3) × (−2) = −6 ✓
  - (+3) + (−2) = +1 ✓
- Step 3: Write as factors: (x + 3)(x − 2)
- **Answer: (x + 3)(x − 2)**

---

**Example 9:** Factorize x² + 8x + 16

**Solution:**
- Step 1: Recognize this is a perfect square (مربع كامل)
- Step 2: Check if it matches a² + 2ab + b²
  - x² + 2(x)(4) + 4² ✓
- Step 3: Factor as (x + 4)²
- **Answer: (x + 4)²**

---

**Example 10:** Factorize 9x² + 9x + 2

**Solution:**
- Step 1: Find two numbers that multiply to 9×2 = 18 and add to 9
- Step 2: The numbers are +3 and +6
- Step 3: Rewrite: 9x² + 3x + 6x + 2
- Step 4: Group: (9x² + 3x) + (6x + 2)
- Step 5: Factor each group: 3x(3x + 1) + 2(3x + 1)
- Step 6: Factor out common term: (3x + 1)(3x + 2)
- **Answer: (3x + 1)(3x + 2)**

---

**Example 11:** Factorize 9x² − 6x + 1

**Solution:**
- Step 1: Recognize this is a perfect square
- Step 2: Check if it matches a² − 2ab + b²
  - (3x)² − 2(3x)(1) + 1² ✓
- Step 3: Factor as (3x − 1)²
- **Answer: (3x − 1)²**

---

**Example 12:** Factorize 5x² − 5

**Solution:**
- Step 1: Factor out common factor 5
- Step 2: 5(x² − 1)
- Step 3: Recognize x² − 1 as difference of squares
- Step 4: 5(x + 1)(x − 1)
- **Answer: 5(x + 1)(x − 1)**

---

**Example 13:** Factorize 3x² − 18x + 27

**Solution:**
- Step 1: Factor out common factor 3
- Step 2: 3(x² − 6x + 9)
- Step 3: Recognize x² − 6x + 9 as perfect square
  - x² − 2(x)(3) + 3² ✓
- Step 4: 3(x − 3)²
- **Answer: 3(x − 3)²**

---

**Example 14:** Factorize 2x² − 12x + 16

**Solution:**
- Step 1: Factor out common factor 2
- Step 2: 2(x² − 6x + 8)
- Step 3: Factor x² − 6x + 8
  - Find numbers that multiply to 8 and add to −6: −2 and −4
- Step 4: 2(x − 2)(x − 4)
- **Answer: 2(x − 2)(x − 4)**

---

### ⚠️ CAUTION: Common Mistakes

**Mistake 1:**
**(a + b)² ≠ a² + b²**

**Correct:**
**(a + b)² = a² + 2ab + b²**

**Example showing the difference:**
- (2 + 3)² = 25
- But 2² + 3² = 4 + 9 = 13 ≠ 25

**Mistake 2:**
**(a − b)² ≠ a² − b²**

**Correct:**
**(a − b)² = a² − 2ab + b²**

---

## 7. Practice Problems with Detailed Solutions

### From Image: Exponent Rules Examples

**Problem (a):** Simplify x⁶x⁻³

**Solution:**
- Step 1: Apply product rule: aᵐ · aⁿ = aᵐ⁺ⁿ
- Step 2: x⁶x⁻³ = x⁶⁺⁽⁻³⁾ = x³
- **Answer: x³**

---

**Problem (b):** Simplify (x⁻¹y²)/(z⁻³)

**Solution:**
- Step 1: Apply negative exponent: z⁻³ = 1/z³
- Step 2: (x⁻¹y²) ÷ (1/z³) = (x⁻¹y²) × z³
- Step 3: Apply negative exponent: x⁻¹ = 1/x
- Step 4: (y²/x) × z³ = y²z³/x
- **Answer: y²z³/x**

---

**Problem (c):** Simplify (x⁻²y³)⁴

**Solution:**
- Step 1: Apply power of a power: (aᵐ)ⁿ = aᵐⁿ
- Step 2: (x⁻²)⁴(y³)⁴ = x⁻⁸y¹²
- Step 3: Apply negative exponent: x⁻⁸ = 1/x⁸
- Step 4: y¹²/x⁸
- **Answer: y¹²/x⁸**

---

**Problem (d):** Simplify (2x²)⁻³ · y⁴ ÷ (x⁻¹y)²

**Solution:**
- Step 1: Simplify (2x²)⁻³
  - (2x²)⁻³ = 2⁻³ · (x²)⁻³ = (1/8) · x⁻⁶ = x⁻⁶/8

- Step 2: Simplify (x⁻¹y)²
  - (x⁻¹y)² = x⁻² · y²

- Step 3: Rewrite expression:
  - (x⁻⁶/8) · y⁴ ÷ (x⁻² · y²)
  - = (x⁻⁶y⁴/8) ÷ (x⁻²y²)
  - = (x⁻⁶y⁴/8) × (1/(x⁻²y²))

- Step 4: Apply quotient rule:
  - = x⁻⁶⁻⁽⁻²⁾ · y⁴⁻² / 8
  - = x⁻⁴ · y² / 8

- Step 5: Apply negative exponent:
  - = y² / (8x⁴)

- **Answer: y²/(8x⁴)**

---

### From Image: Expansion Problems

**Problem 1(a):** Expand (2x + 3)²

**Solution:**
- Step 1: Use (a + b)² = a² + 2ab + b²
- Step 2: a = 2x, b = 3
- Step 3: (2x)² + 2(2x)(3) + 3²
- Step 4: 4x² + 12x + 9
- **Answer: 4x² + 12x + 9**

---

**Problem 1(b):** Expand (3x − y)²

**Solution:**
- Step 1: Use (a − b)² = a² − 2ab + b²
- Step 2: a = 3x, b = y
- Step 3: (3x)² − 2(3x)(y) + y²
- Step 4: 9x² − 6xy + y²
- **Answer: 9x² − 6xy + y²**

---

**Problem 1(c):** Expand (x + 3y)(x − 3y)

**Solution:**
- Step 1: Use (a + b)(a − b) = a² − b²
- Step 2: a = x, b = 3y
- Step 3: x² − (3y)²
- Step 4: x² − 9y²
- **Answer: x² − 9y²**

---

**Problem 1(d):** Expand (x + 3y)(x + 4y)

**Solution:**
- Step 1: Use FOIL method
- Step 2: First: x · x = x²
- Step 3: Outer: x · 4y = 4xy
- Step 4: Inner: 3y · x = 3xy
- Step 5: Last: 3y · 4y = 12y²
- Step 6: Combine: x² + 4xy + 3xy + 12y²
- Step 7: x² + 7xy + 12y²
- **Answer: x² + 7xy + 12y²**

---

**Problem 1(e):** Expand (2√x − 3)²

**Solution:**
- Step 1: Use (a − b)² = a² − 2ab + b²
- Step 2: a = 2√x, b = 3
- Step 3: (2√x)² − 2(2√x)(3) + 3²
- Step 4: 4x − 12√x + 9
- **Answer: 4x − 12√x + 9**

---

**Problem 1(f):** Expand (√x + 5)(√x − 5)

**Solution:**
- Step 1: Use (a + b)(a − b) = a² − b²
- Step 2: a = √x, b = 5
- Step 3: (√x)² − 5²
- Step 4: x − 25
- **Answer: x − 25**

---

### From Image: Factorization Problems

**Problem 2(a):** Factorize x² − 7x + 12

**Solution:**
- Step 1: Find two numbers that multiply to 12 and add to −7
- Step 2: Numbers: −3 and −4
  - (−3)(−4) = 12 ✓
  - −3 + (−4) = −7 ✓
- Step 3: (x − 3)(x − 4)
- **Answer: (x − 3)(x − 4)**

---

**Problem 2(b):** Factorize x² + x − 6

**Solution:**
- Step 1: Find two numbers that multiply to −6 and add to 1
- Step 2: Numbers: 3 and −2
  - (3)(−2) = −6 ✓
  - 3 + (−2) = 1 ✓
- Step 3: (x + 3)(x − 2)
- **Answer: (x + 3)(x − 2)**

---

**Problem 2(c):** Factorize x² + 8x + 16

**Solution:**
- Step 1: Recognize as perfect square
- Step 2: x² + 2(x)(4) + 4²
- Step 3: (x + 4)²
- **Answer: (x + 4)²**

---

**Problem 2(d):** Factorize 9x² + 9x + 2

**Solution:**
- Step 1: Product = 9 × 2 = 18, Sum = 9
- Step 2: Numbers: 3 and 6
- Step 3: 9x² + 3x + 6x + 2
- Step 4: 3x(3x + 1) + 2(3x + 1)
- Step 5: (3x + 1)(3x + 2)
- **Answer: (3x + 1)(3x + 2)**

---

**Problem 2(e):** Factorize 9x² − 6x + 1

**Solution:**
- Step 1: Recognize as perfect square
- Step 2: (3x)² − 2(3x)(1) + 1²
- Step 3: (3x − 1)²
- **Answer: (3x − 1)²**

---

**Problem 2(f):** Factorize 5x² − 5

**Solution:**
- Step 1: Factor out 5
- Step 2: 5(x² − 1)
- Step 3: Recognize difference of squares
- Step 4: 5(x + 1)(x − 1)
- **Answer: 5(x + 1)(x − 1)**

---

**Problem 2(g):** Factorize 3x² − 18x + 27

**Solution:**
- Step 1: Factor out 3
- Step 2: 3(x² − 6x + 9)
- Step 3: Recognize perfect square
- Step 4: 3(x − 3)²
- **Answer: 3(x − 3)²**

---

**Problem 2(h):** Factorize 2x² − 12x + 16

**Solution:**
- Step 1: Factor out 2
- Step 2: 2(x² − 6x + 8)
- Step 3: Find numbers: −2 and −4
- Step 4: 2(x − 2)(x − 4)
- **Answer: 2(x − 2)(x − 4)**

---

### From Image: Simplification Problems

**Problem 3(a):** Simplify (x² − x − 6)/(x² − 7x + 12)

**Solution:**
- Step 1: Factorize numerator: x² − x − 6
  - Numbers: −3 and 2 (multiply to −6, add to −1)
  - (x − 3)(x + 2)

- Step 2: Factorize denominator: x² − 7x + 12
  - Numbers: −3 and −4 (multiply to 12, add to −7)
  - (x − 3)(x − 4)

- Step 3: Simplify:
  - [(x − 3)(x + 2)] / [(x − 3)(x − 4)]
  - Cancel (x − 3)
  - (x + 2)/(x − 4)

- **Answer: (x + 2)/(x − 4)**

---

**Problem 3(b):** Simplify (x² + 3x − 4)/(2 − x − x²)

**Solution:**
- Step 1: Factorize numerator: x² + 3x − 4
  - Numbers: 4 and −1
  - (x + 4)(x − 1)

- Step 2: Factorize denominator: 2 − x − x²
  - Rearrange: −x² − x + 2 = −(x² + x − 2)
  - Factor: −(x + 2)(x − 1)

- Step 3: Simplify:
  - [(x + 4)(x − 1)] / [−(x + 2)(x − 1)]
  - Cancel (x − 1)
  - (x + 4) / [−(x + 2)]
  - −(x + 4)/(x + 2)

- **Answer: −(x + 4)/(x + 2)**

---

**Problem 3(c):** Simplify (2x)/(x² − 1) ÷ (4x² + 4x)/(x − 1)

**Solution:**
- Step 1: Change division to multiplication:
  - (2x)/(x² − 1) × (x − 1)/(4x² + 4x)

- Step 2: Factorize:
  - x² − 1 = (x + 1)(x − 1)
  - 4x² + 4x = 4x(x + 1)

- Step 3: Substitute:
  - [2x / ((x + 1)(x − 1))] × [(x − 1) / (4x(x + 1))]

- Step 4: Simplify:
  - [2x(x − 1)] / [(x + 1)(x − 1) · 4x(x + 1)]
  - Cancel x and (x − 1)
  - 2 / [4(x + 1)²]
  - 1 / [2(x + 1)²]

- **Answer: 1/[2(x + 1)²]**

---

**Problem 3(d):** Simplify [1/(x + h) − 1/x] / h

**Solution:**
- Step 1: Find common denominator for numerator:
  - 1/(x + h) − 1/x = [x − (x + h)] / [x(x + h)]
  - = (x − x − h) / [x(x + h)]
  - = −h / [x(x + h)]

- Step 2: Divide by h:
  - [−h / (x(x + h))] ÷ h
  - = [−h / (x(x + h))] × (1/h)

- Step 3: Simplify:
  - −h / [hx(x + h)]
  - Cancel h
  - −1 / [x(x + h)]

- **Answer: −1/[x(x + h)]**

---

## Summary 

This section sheet covered:

1. **Mathematical Symbols** with English and Arabic names
2. **Real Line** representation of real numbers
3. **Properties of Real Numbers** (Commutative, Associative, Identity, Inverse, Distributive)
4. **Order Relations and Intervals** (Open, Closed, Half-open, Infinite)
5. **Exponents and Radicals** with 8 key rules
6. **Algebraic Identities** including squares and difference of squares
7. **Detailed Practice Problems** with step-by-step solutions

---

## Tips for Success 

1. **Practice regularly** - Mathematics requires consistent practice
2. **Memorize the identities** - They are fundamental tools
3. **Check your work** - Always verify your answers by substitution
4. **Factor first** - In simplification problems, always factor before canceling
5. **Watch for common mistakes** - Remember (a + b)² ≠ a² + b²

---

**Good Luck! **

---

*End of Section Sheet*

